src/verification/dafny/astar_navfnplanner-go/src/main.go
@@ -1,0 +1,180 @@
+/**
+ * Entry point for the Dafny implementation of ROS' NavFn planner.
+ *
+ * It loads the map and test cases from the input file and
+ * runs the AStar function generated from the Dafny code.
+ */
+
+package main
+
+import (
+	"astar_navfnplanner/dafny"
+	"bufio"
+	"errors"
+	"fmt"
+	"io"
+	"os"
+	"path/filepath"
+	"strconv"
+	"strings"
+)
+
+func Max(x, y int) int {
+    if x < y {
+        return y
+    }
+    return x
+}
+
+func printPath(path dafny.Seq) {
+	it := path.Iterator()
+
+	elem, has := it()
+
+	if has {
+		dx, dy := elem.(RealPoint).Dtor_col(), elem.(RealPoint).Dtor_row()
+
+		fmt.Printf("[%g, %g]", dx.Float64(), dy.Float64())
+		elem, has := it()
+
+		for has {
+			dx, dy := elem.(RealPoint).Dtor_col(), elem.(RealPoint).Dtor_row()
+
+			fmt.Printf(", [%g, %g]", dx.Float64(), dy.Float64())
+			elem, has = it()
+		}
+	}
+}
+
+func printNavfn(navfn dafny.Seq) {
+	for i := 0; i < navfn.LenInt(); i++ {
+		row := navfn.IndexInt(i).(dafny.Seq)
+		for j := 0;  j < row.LenInt(); j++ {
+			value_raw := row.IndexInt(j).(RealInf);
+			value := 1e10
+			if value_raw.Is_Real() {
+				value = value_raw.Dtor_r().Float64()
+			}
+			if i == 0 && j == 0 {
+				fmt.Printf("%g", value)
+			} else {
+				fmt.Printf(", %g", value)
+			}
+		}
+	}
+}
+
+func readFile(reader io.Reader, base string, printNavFn bool) (error) {
+	scanner := bufio.NewReader(reader)
+
+	// Width
+	width_s, err := scanner.ReadString(' ')
+
+	if err != nil {
+		return errors.New("width expected, nothing found")
+	}
+
+	width, err := strconv.Atoi(strings.TrimSpace(width_s))
+
+	if err != nil {
+		return err
+	}
+
+	// Height
+	height_s, err := scanner.ReadString('\n')
+
+	if err != nil {
+		return errors.New("height expected, nothing found")
+	}
+
+	height, err := strconv.Atoi(strings.TrimSpace(height_s))
+
+	if err != nil {
+		return err
+	}
+
+	// Filename
+	filename, err := scanner.ReadString('\n')
+
+	if err != nil {
+		return errors.New("file name expected, nothing found")
+	}
+
+	costmap, err := os.ReadFile(filepath.Join(base, strings.TrimSpace(filename)))
+
+	if err != nil {
+		return err
+	}
+
+	// Test cases
+	line, err := scanner.ReadString('\n')
+
+	for err == nil {
+		positions_s := strings.Split(strings.TrimSpace(line), " ")
+
+		if len(positions_s) > 1 && positions_s[0] != "-1" {
+			var positions [4]int
+
+			for i := 0; i < 4; i++ {
+				positions[i], err = strconv.Atoi(positions_s[i])
+
+				if err != nil {
+					return err
+				}
+			}
+
+			start := Companion_Pose_.Create_Pose_(Companion_Point_.Create_Point_(dafny.IntOf(positions[1]), dafny.IntOf(positions[0])))
+			goal := Companion_Pose_.Create_Pose_(Companion_Point_.Create_Point_(dafny.IntOf(positions[3]), dafny.IntOf(positions[2])))
+			costMap := Companion_CostMap_.Create_CostMap_(func (p Point) dafny.Real {
+				index := p.Dtor_col().Int() + p.Dtor_row().Int() * width
+				return dafny.RealOf(float64(int(costmap[index])))
+			}, dafny.IntOf(height), dafny.IntOf(width))
+			numIterations := dafny.IntOf(Max(width * height / 20, width + height))
+			numPathIterations := dafny.IntOf(4 * width)
+
+			// The complete AStar algorithm
+			err, path, navfn := Companion_Default___.AStar(start, goal, costMap, numIterations, numPathIterations)
+
+			// Print a JSON object
+			fmt.Printf("{\"initial\": [%d, %d], \"goal\": [%d, %d], ", positions[0], positions[1], positions[2], positions[3])
+
+			if err {
+				path = dafny.EmptySeq
+			}
+
+			fmt.Print("\"path\": [")
+			printPath(path)
+			if printNavFn {
+				fmt.Print("], \"navfn\": [")
+				printNavfn(navfn)
+			}
+			fmt.Println("]}")
+		}
+
+		line, err = scanner.ReadString('\n')
+	}
+
+	return nil
+}
+
+func main() {
+	filename := os.Args[1]
+	printNavFn := true
+
+	if filename == "--no-navfn" {
+		filename = os.Args[2]
+		printNavFn = false
+	}
+
+	file, err := os.Open(filename)
+
+	if err != nil {
+		panic(err)
+	}
+
+	err = readFile(file, filepath.Dir(filename), printNavFn)
+
+	if err != nil {
+		panic(err)
+	}
+}
